README.md
@@ -13,7 +13,7 @@ This version is known to compile with:
 ## Building from source
 
 When building from source, we recommend to use opam (2.0.0 or newer) for
-installing the dependencies.  This requires the following two repositories:
+installing the dependencies. This requires the following two repositories:
 
     opam repo add coq-released https://coq.inria.fr/opam/released
     opam repo add iris-dev https://gitlab.mpi-sws.org/iris/opam.git
@@ -24,37 +24,37 @@ of the dependencies.
 Run `make -jN` to build the full development, where `N` is the number of your
 CPU cores.
 
-To update, do `git pull`.  After an update, the development may fail to compile
-because of outdated dependencies.  To fix that, please run `opam update`
+To update, do `git pull`. After an update, the development may fail to compile
+because of outdated dependencies. To fix that, please run `opam update`
 followed by `make build-dep`.
 
 ## Structure
 
-* The folder [util](theories/util) contains utility for basic concepts.
-  * [fancy_lists.v](theories/util/fancy_lists.v) contains definitions, notation
+- The folder [util](theories/util) contains utility for basic concepts.
+  - [fancy_lists.v](theories/util/fancy_lists.v) contains definitions, notation
     and lemmas for heterogeneous lists and related data types.
-* The folder [prophecy](theories/prophecy) contains the prophecy library,
+- The folder [prophecy](theories/prophecy) contains the prophecy library,
   as well as the library for syntactic types.
-* The folder [lifetime](theories/lifetime) proves the rules of the lifetime
+- The folder [lifetime](theories/lifetime) proves the rules of the lifetime
   logic, including derived constructions like (non-)atomic persistent borrows.
-  * The subfolder [model](theories/lifetime/model) proves the core rules, which
+  - The subfolder [model](theories/lifetime/model) proves the core rules, which
     are then sealed behind a module signature in
     [lifetime.v](theories/lifetime/lifetime.v).
-* The folder [lang](theories/lang) contains the formalization of the lambda-Rust
+- The folder [lang](theories/lang) contains the formalization of the lambda-Rust
   core language, including the theorem showing that programs with data races get
   stuck.
-* The folder [typing](theories/typing) defines the domain of semantic types and
+- The folder [typing](theories/typing) defines the domain of semantic types and
   interpretations of all the judgments and also proves all typing rules.
-  * [type.v](theories/typing/type.v) contains the definition of the notion
+  - [type.v](theories/typing/type.v) contains the definition of the notion
     of the semantic type.
-  * [programs.v](theories/typing/programs.v) defines the typing judgments for
+  - [programs.v](theories/typing/programs.v) defines the typing judgments for
     instructions and function bodies.
-  * [soundness.v](theories/typing/soundness.v) contains the main soundness
+  - [soundness.v](theories/typing/soundness.v) contains the main soundness
     (adequacy) theorem of the type system.
-  * The subfolder [examples](theories/typing/examples) verifies some example
+  - The subfolder [examples](theories/typing/examples) verifies some example
     Rust programs in Coq to conceptually demonstrate how functional verification
     works under the RustHorn-style translation.
-  * The subfolder [lib](theories/typing/lib) contains proofs for some APIs
+  - The subfolder [lib](theories/typing/lib) contains proofs for some APIs
     with unsafe code from the Rust standard library and some user crates.
     Some libraries are not yet verified, being commented out in `_CoqProject`.
 
@@ -93,7 +93,7 @@ The filenames are spread across `theories/typing/examples`, `theories/typing`, `
 | `pop`               | `vec_pushpop.v`   | `vec_pop_type`           |
 | `index_mut`         | `vec_index.v`     | `vec_index_uniq_type`    |
 | **`IterMut`**       |                   |                          |
-| `iter_mut`          | `vec_slice.v`     | `vec_to_uniq_slice_type` |
+| `iter_mut`          | `vec_slice.v`     | `vec_as_slice_uniq_type` |
 | `next`              | `iter.v`          | `iter_uniq_next_type`    |
 | `inc_vec`           | `inc_vec.v`       | `inc_vec_type`           |
 | **`Cell`**          |                   |                          |
@@ -103,48 +103,48 @@ The filenames are spread across `theories/typing/examples`, `theories/typing`, `
 | `inc_cell`          | `inc_cell.v`      | `inc_cell_type`          |
 | **`Mutex`**         |                   |                          |
 | `new`               | `mutex.v`         | `mutex_new_type`         |
-| `get_mut`           | `mutex.v`         | `mutex_get_mut`          |
+| `get_mut`           | `mutex.v`         | `mutex_get_uniq`          |
 
 ### Key Type(-Spec) Rules --- from the RustBelt Paper
 
 The files in [typing](theories/typing) prove semantic versions of the proof
-rules given in the *RustBelt* paper.  Notice that mutable borrows are called
+rules given in the _RustBelt_ paper. Notice that mutable borrows are called
 "unique borrows" in the Coq development.
 
-| Proof Rule            | File            | Lemma                 |
-|-----------------------|-----------------|-----------------------|
-| T-bor-lft (for shr)   | shr_bor.v       | shr_subtype           |
-| T-bor-lft (for mut)   | uniq_bor.v      | uniq_subtype          |
-| C-subtype             | type_context.v  | subtype_tctx_incl     |
-| C-copy                | type_context.v  | copy_tctx_incl        |
-| C-split-bor (for shr) | product_split.v | tctx_split_shr_prod   |
-| C-split-bor (for mut) | product_split.v | tctx_split_uniq_prod  |
-| C-share               | borrow.v        | tctx_share            |
-| C-borrow              | borrow.v        | tctx_borrow           |
-| C-reborrow            | uniq_bor.v      | tctx_reborrow_uniq    |
-| Tread-own-copy        | own.v           | read_own_copy         |
-| Tread-own-move        | own.v           | read_own_move         |
-| Tread-bor (for shr)   | shr_bor.v       | read_shr              |
-| Tread-bor (for mut)   | uniq_bor.v      | read_uniq             |
-| Twrite-own            | own.v           | write_own             |
-| Twrite-bor            | uniq_bor.v      | write_uniq            |
-| S-num                 | int.v           | type_int_instr        |
-| S-nat-leq             | int.v           | type_le_instr         |
-| S-new                 | own.v           | type_new_instr        |
-| S-delete              | own.v           | type_delete_instr     |
-| S-deref               | programs.v      | type_deref_instr      |
-| S-assign              | programs.v      | type_assign_instr     |
-| F-consequence         | programs.v      | typed_body_impl       |
-| F-let                 | programs.v      | type_let'             |
-| F-letcont             | cont.v          | type_cont             |
-| F-jump                | cont.v          | type_jump             |
-| F-newlft              | programs.v      | type_newlft           |
-| F-endlft              | programs.v      | type_endlft           |
-| F-call                | function.v      | type_call             |
+| Proof Rule            | File            | Lemma                |
+| --------------------- | --------------- | -------------------- |
+| T-bor-lft (for shr)   | shr_bor.v       | shr_subtype          |
+| T-bor-lft (for mut)   | uniq_bor.v      | uniq_subtype         |
+| C-subtype             | type_context.v  | subtype_tctx_incl    |
+| C-copy                | type_context.v  | copy_tctx_incl       |
+| C-split-bor (for shr) | product_split.v | tctx_split_shr_prod  |
+| C-split-bor (for mut) | product_split.v | tctx_split_uniq_prod |
+| C-share               | borrow.v        | tctx_share           |
+| C-borrow              | borrow.v        | tctx_borrow          |
+| C-reborrow            | uniq_bor.v      | tctx_reborrow_uniq   |
+| Tread-own-copy        | own.v           | read_own_copy        |
+| Tread-own-move        | own.v           | read_own_move        |
+| Tread-bor (for shr)   | shr_bor.v       | read_shr             |
+| Tread-bor (for mut)   | uniq_bor.v      | read_uniq            |
+| Twrite-own            | own.v           | write_own            |
+| Twrite-bor            | uniq_bor.v      | write_uniq           |
+| S-num                 | int.v           | type_int_instr       |
+| S-nat-leq             | int.v           | type_le_instr        |
+| S-new                 | own.v           | type_new_instr       |
+| S-delete              | own.v           | type_delete_instr    |
+| S-deref               | programs.v      | type_deref_instr     |
+| S-assign              | programs.v      | type_assign_instr    |
+| F-consequence         | programs.v      | typed_body_impl      |
+| F-let                 | programs.v      | type_let'            |
+| F-letcont             | cont.v          | type_cont            |
+| F-jump                | cont.v          | type_jump            |
+| F-newlft              | programs.v      | type_newlft          |
+| F-endlft              | programs.v      | type_endlft          |
+| F-call                | function.v      | type_call            |
 
 Some of these lemmas are called `something'` because the version without the
 `'` is a derived, more specialized form used together with our `eauto`-based
-`solve_typing` tactic.  You can see this tactic in action in the
+`solve_typing` tactic. You can see this tactic in action in the
 [examples](theories/typing/examples) subfolder.
 
 ### Lifetime Logic Rules
@@ -155,7 +155,7 @@ then sealed behind a module signature in
 [lifetime.v](theories/lifetime/lifetime.v).
 
 | Proof Rule        | File                | Lemma                |
-|-------------------|---------------------|----------------------|
+| ----------------- | ------------------- | -------------------- |
 | LftL-begin        | model/creation.v    | lft_create           |
 | LftL-tok-fract    | model/primitive.v   | lft_tok_fractional   |
 | LftL-not-own-end  | model/primitive.v   | lft_tok_dead         |
@@ -178,10 +178,10 @@ then sealed behind a module signature in
 
 ## For Developers: How to update the Iris dependency
 
-* Do the change in Iris, push it.
-* Wait for CI to publish a new Iris version on the opam archive, then run
+- Do the change in Iris, push it.
+- Wait for CI to publish a new Iris version on the opam archive, then run
   `opam update iris-dev`.
-* In lambdaRust, change the `opam` file to depend on the new version.
-* Run `make build-dep` (in lambdaRust) to install the new version of Iris.
+- In lambdaRust, change the `opam` file to depend on the new version.
+- Run `make build-dep` (in lambdaRust) to install the new version of Iris.
   You may have to do `make clean` as Coq will likely complain about `.vo` file
   mismatches.
